First-cut version with reverse transition function and proofs.

src/dafny/utils/Automata.dfy
@@ -44,6 +44,7 @@ module Automata {
   datatype Auto<!T(!new,==)> =
     Auto(ghost transitions: map<T, seq<T>> := map[],
          transitionsNat: map<nat, seq<nat>> := map[],
+         revTransitionsNat: map<nat, seq<nat>> := map[],
          states: seq<T> := [],
          indexOf: map<T, nat> := map[])
   {
@@ -59,23 +60,30 @@ module Automata {
       */
     function {:timeLimitMultiplier 8} {:opaque} AddState(i: T): (a: ValidAuto<T>)
       requires IsValid()
+      requires IsReversemapValid()
       ensures i in a.states
       ensures forall s:: s in states ==> s in a.states
       ensures forall s:: s in a.states ==> s in states || s == i
       ensures i in states ==> a == this
       ensures i !in states ==> a.SSize() == SSize() + 1
       ensures i !in states ==> (forall s:: s in states ==> a.transitions[s] == transitions[s]) && a.transitions[i] == []
+      ensures i !in states ==> a.transitionsNat[|states|] == []
+      ensures i !in states ==> a.revTransitionsNat[|states|] == []
       ensures a.IsValid()
+      ensures a.IsReversemapValid()
     {
       if i in states then
         this
       else
+        assert i !in indexOf;
         assert (indexOf + map[i := |states|]).Values == indexOf.Values + { |states| };
-        this
-        .(states := states + [i])
-        .(indexOf := indexOf + map[i := |states|])
-        .(transitions := transitions + map[i := []])
-        .(transitionsNat := transitionsNat + map[|states| := []])
+        assert indexOf[i := |states|] == indexOf + map[i := |states|];
+        this.(
+        states := states + [i],
+        indexOf := indexOf[i := |states|],
+        transitions := transitions[i := []],
+        transitionsNat := transitionsNat[|states| := []],
+        revTransitionsNat := revTransitionsNat[|states| := []])
     }
 
     /**
@@ -83,6 +91,7 @@ module Automata {
       */
     function {:opaque} AddStates(xs: seq<T>): (a: ValidAuto<T>)
       requires IsValid()
+      requires IsReversemapValid()
       ensures a.IsValid()
       ensures forall s:: s in states ==> s in a.states
       ensures forall j:: 0 <= j < |xs| ==> xs[j] in a.states
@@ -103,60 +112,269 @@ module Automata {
       */
     function {:timeLimitMultiplier 8} {:opaque} AddEdge(i: T, j: T): (a: ValidAuto<T>)
       requires IsValid()
+      requires IsReversemapValid()
+
       ensures i in a.states
       ensures j in a.states
       ensures forall s:: s in states ==> s in a.states
       ensures forall s:: s in a.states ==> s in states || s == i || s == j
+      ensures forall s:: s in a.states && s != i && s != j ==> s in a.transitions
       ensures forall s:: s in a.states && s != i && s != j ==> a.transitions[s] == transitions[s]
+      ensures i in a.transitions
       ensures i in states ==> |a.transitions[i]| <= |transitions[i]| + 1
       ensures i !in states ==> a.transitions[i] == [j]
+      ensures a.IsReversemapValid()
     {
       var a1 := this.AddState(i).AddState(j);
-      assert i in a1.states;
-      assert j in a1.states;
       if a1.indexOf[j] in a1.transitionsNat[a1.indexOf[i]] then
         assert j in a1.transitions[i];
         a1
       else
         AddEdgeInTRandTrNatPreservesValid(a1, i, j);
-        var w :=
-          a1
-          .(transitions := a1.transitions + map[i := a1.transitions[i] + [j]])
-          .(transitionsNat := a1.transitionsNat + map[a1.indexOf[i] := a1.transitionsNat[a1.indexOf[i]] + [a1.indexOf[j]]]);
+        var w := a1.(transitions := AddKeyVal2(a1.transitions, i, j),
+                 transitionsNat := AddKeyVal(a1.transitionsNat, a1.indexOf[i], a1.indexOf[j]),
+                 revTransitionsNat := AddKeyVal(a1.revTransitionsNat, a1.indexOf[j], a1.indexOf[i]));
         w
     }
 
     /** A lemma to make verification of AddEdge easier. */
-    lemma AddEdgeInTRandTrNatPreservesValid(a: ValidAuto<T>, i: T, j: T)
+    lemma {:timeLimitMultiplier 6} AddEdgeInTRandTrNatPreservesValid(a: ValidAuto<T>, i: T, j: T)
       requires a.IsValid()
+      requires a.IsReversemapValid()
       requires i in a.states
       requires j in a.states
       ensures a
-              .(transitions := a.transitions + map[i := a.transitions[i] + [j]])
-              .(transitionsNat := a.transitionsNat + map[a.indexOf[i] := a.transitionsNat[a.indexOf[i]] + [a.indexOf[j]]]).IsValid()
-    {   //  Thanks Dafny 
+              .(transitions := AddKeyVal2(a.transitions, i, j))
+              .(transitionsNat := AddKeyVal(a.transitionsNat, a.indexOf[i], a.indexOf[j]))
+              .(revTransitionsNat := AddKeyVal(a.revTransitionsNat, a.indexOf[j], a.indexOf[i]))
+              .IsValid()
+      ensures var a1 := a
+                        .(transitions := AddKeyVal2(a.transitions, i, j),
+                        transitionsNat := AddKeyVal(a.transitionsNat, a.indexOf[i], a.indexOf[j]),
+                        revTransitionsNat := AddKeyVal(a.revTransitionsNat, a.indexOf[j], a.indexOf[i]));
+              a1.IsReversemapValid()
+    {
+      var a1 := a.(transitions := AddKeyVal2(a.transitions, i, j));
+      assert a1.transitionsNat == a.transitionsNat;
+      assert a1.revTransitionsNat == a.revTransitionsNat;
+      foo303(a, a1);
+      assert a1.IsReversemapValid();
+      var a2 := a1.(
+      transitionsNat := AddKeyVal(a1.transitionsNat, a.indexOf[i], a.indexOf[j]),
+      revTransitionsNat := AddKeyVal(a1.revTransitionsNat, a.indexOf[j], a.indexOf[i]));
+      assert a2.transitionsNat == AddKeyVal(a1.transitionsNat, a.indexOf[i], a.indexOf[j]);
+      assert a2.revTransitionsNat == AddKeyVal(a1.revTransitionsNat, a.indexOf[j], a.indexOf[i]);
+      foo(a1.transitionsNat, a1.revTransitionsNat, a.indexOf[i], a.indexOf[j]);
+      assert a2.IsReversemapValid();
     }
+
+    // lemma {:timeLimitMultiplier 2} foo202(i: T, j: T)
+    //   requires i in transitions
+    //   requires j in transitions
+    //   requires IsReversemapValid()
+    //   ensures
+    //     var a1 := this.(transitions := AddKeyVal2(this.transitions, i, j));
+    //     a1.IsReversemapValid()
+    // {
+    //   var a1 := this.(transitions := AddKeyVal2(this.transitions, i, j));
+    //   assert a1.transitionsNat == this.transitionsNat;
+    //   assert a1.revTransitionsNat == this.revTransitionsNat;
+    //   foo303(this, a1);
+    //   assert a1.IsReversemapValid();
+
+    // }
+
+    static lemma foo303(a: Auto<T>, b: Auto<T>)
+      requires a.IsReversemapValid()
+      requires a.transitionsNat == b.transitionsNat
+      requires a.revTransitionsNat == b.revTransitionsNat
+      ensures b.IsReversemapValid()
+    {
+      forall src, tgt | src in b.transitionsNat && tgt in b.transitionsNat[src]
+        ensures tgt in b.revTransitionsNat && src in b.revTransitionsNat[tgt]
+      {
+        assert tgt in a.revTransitionsNat && src in a.revTransitionsNat[tgt];
+        assert a.revTransitionsNat == b.revTransitionsNat;
+        assert tgt in b.revTransitionsNat && src in b.revTransitionsNat[tgt];
+      }
+      forall src, tgt | src in b.revTransitionsNat && tgt in b.revTransitionsNat[src]
+        ensures tgt in b.transitionsNat && src in b.transitionsNat[tgt]
+      {
+        assert tgt in a.transitionsNat && src in a.transitionsNat[tgt];
+        assert a.transitionsNat == b.transitionsNat;
+        assert tgt in b.transitionsNat && src in b.transitionsNat[tgt];
+      }
+    }
+
+    static lemma foo(m: map<nat, seq<nat>>, m': map<nat, seq<nat>>, i: nat, j: nat)
+      //   requires m.Keys == m'.Keys
+      requires i in m
+      requires j in m
+      requires IsReversemap(m, m')
+      ensures IsReversemap(AddKeyVal(m, i, j), AddKeyVal(m', j, i))
+    {
+
+    }
+
+    // static lemma foo2<T(==)>(m: map<T, seq<T>>, m': map<T, seq<T>>, i: T, j: T)
+    //   requires m.Keys == m'.Keys
+    //   requires i in m
+    //   requires j in m
+    //   requires IsReversemap2(m, m')
+    //   ensures IsReversemap2(AddKeyVal2(m, i, j), AddKeyVal2(m', j, i))
+    // {
+
+    // }
+
+    static function AddKeyVal(m: map<nat, seq<nat>>, key: nat, val: nat): (m': map<nat, seq<nat>>)
+      requires key in m
+    {
+      m[key := m[key] + [val]]
+    }
+
+    static function AddKeyVal2<T(==)>(m: map<T, seq<T>>, key: T, val: T): (m': map<T, seq<T>>)
+      requires key in m
+      requires val in m
+    {
+      m[key := m[key] + [val]]
+    }
+
 
     /**
       *  Add several transitions from i to all the elements of js.
       */
-    function {:timeLimitMultiplier 4} {:opaque} AddEdges(i: T, js: seq<T>, index: nat := 0): (a: ValidAuto<T>)
+    function {:timeLimitMultiplier 6} {:opaque} AddEdges(i: T, js: seq<T>, index: nat := 0): (a: ValidAuto<T>)
       requires this.IsValid()
+        requires IsReversemapValid()
       requires index <= |js|
       requires forall j:: 0 <= j < index ==> js[j] in this.states
       ensures a.IsValid()
+      ensures a.IsReversemapValid()
       ensures i in a.states
       ensures forall s:: s in this.states ==> s in a.states
       ensures forall j:: 0 <= j < |js| ==> js[j] in a.states
       ensures forall s:: s in a.states ==> s in this.states || s == i || s in js
       decreases |js| - index
     {
-      if |js| == index then this.AddState(i)
+    //   assume this.IsReversemapValid();
+      if |js| == index then
+        this.AddState(i)
       else
-        var a1 := this.AddEdge(i, js[index]);
+        // assume this.AddEdge.requires(i, js[index]);
+        var a1: ValidAuto<T> := this.AddEdge(i, js[index]);
+        assert i in a1.states;
+        assert js[index] in a1.states;
+        assert a1.IsValid();
+        // // assume a1.IsReversemapValid();
+        // assume a1.AddEdges.requires(i, js, index + 1);
+        // assume a1.IsValid();
+        assert  forall j:: 0 <= j < index  ==> js[j] in a1.states;
+        assert js[index] in a1.states;
+        foo404(index, js, a1.states);
+        assert forall j:: 0 <= j < index + 1 ==> js[j] in a1.states;
         var a2 := a1.AddEdges(i, js, index + 1);
+        // assume a2.IsValid();
+        // assume a2.IsReversemapValid();
+        // a2
         a2
     }
+
+    static lemma foo404(index: nat, js: seq<T>, b: seq<T>)
+      requires index < |js|
+      requires  forall j:: 0 <= j < index  ==> js[j] in b
+      requires js[index] in b
+      ensures forall j:: 0 <= j < index + 1 ==> js[j] in b
+    {
+
+    }
+
+    /**
+      *  Add edges from each j in js to i 
+      */
+    // function {:timeLimitMultiplier 4} {:opaque} AddReverseEdges(i: T, js: seq<T>, index: nat := 0): (a: ValidAuto<T>)
+    //   requires this.IsValid()
+    //   requires index <= |js|
+    //   requires forall j:: 0 <= j < |js| ==> js[j] in this.states
+    //   requires i in states
+    //   requires forall j:: 0 <= j < index ==> i in transitions[js[j]]
+    //   //   requires forall j, tgt:: 0 <= j < index && tgt in transitions[states[j]] ==> (states[j] in transitions[tgt])
+
+    //   ensures a.IsValid()
+    //   ensures a.states == this.states
+    //   ensures forall t:: t in a.transitions <==> t in this.transitions || (t in js && i in transitions[t])
+    //   ensures forall j:: j in js ==> j in a.transitions
+    //   ensures forall j:: 0 <= j < |js| ==> i in a.transitions[js[j]]
+    //   //   ensures forall j, tgt:: 0 <= j < |js| && tgt in transitions[states[j]] ==> (states[j] in a.transitions[tgt])
+
+    //   decreases |js| - index
+    // {
+    //   reveal_AddEdge();
+    //   if |js| == index then this
+    //   else
+    //     var a1 := this.AddEdge(js[index], i);
+    //     a1.AddReverseEdges(i, js, index + 1)
+    // }
+
+    // function {:timeLimitMultiplier 4} {:opaque} AddReverseEdges2(i: nat, js: seq<nat>, index: nat := 0): (a: Auto<T>)
+    //   requires this.IsValid()
+    //   requires i in transitionsNat
+    //   requires index <= |js|
+    // //   requires
+    // //   requires forall j:: 0 <= j < |js| ==> js[j] in this.states
+    // //   requires i in states
+    // //   requires forall j:: 0 <= j < index ==> i in transitions[js[j]]
+    // //   requires forall j, tgt:: 0 <= j < index && tgt in transitions[states[j]] ==> (states[j] in transitions[tgt])
+
+    // //   ensures a.IsValid()
+    //   ensures a.states == this.states
+    // //   ensures forall t:: t in a.transitions <==> t in this.transitions || (t in js && i in transitions[t])
+    // //   ensures forall j:: j in js ==> j in a.transitions
+    // //   ensures forall j:: 0 <= j < |js| ==> i in a.transitions[js[j]]
+    // //   ensures forall j, tgt:: 0 <= j < |js| && tgt in transitions[states[j]] ==> (states[j] in a.transitions[tgt])
+
+    //   decreases |js| - index
+    // {
+    //   reveal_AddEdge();
+    //   if index == |js| then this
+    //   else
+    //     // var forwardTrans := if indextransitionsNat[index] else [];
+    //     var a1 := this.(transitionsNat := transitionsNat[index := transitionsNat[index] + [i]]);
+    //     assume a1.IsValid();
+    //     a1.AddReverseEdges2(i, js, index + 1)
+    // }
+
+    // function ReverseMap(m: map<nat, seq<nat>>, index: nat := 0): (m': map<nat, seq<nat>>)
+    //   requires forall k:: k in m <==> 0 <= k < |m|
+    // {
+    //   m
+    // }
+
+    // function AddReverseEntries(m: map<nat, seq<nat>>, k: nat, xe: seq<nat>, b: nat): (m': map<nat, seq<nat>>)
+    //   requires forall key:: key in m <==> 0 <= key < b
+    //   requires forall i:: 0 <= i < |xe| ==> 0 <= xe[i] < b
+    //   requires forall  key, i:: key in m && 0 <= i < |m[key]| ==> 0 <= m[key][i] < b
+    //   requires k < b
+    //   //  tuples of m are preserved
+    //   ensures forall key, val:: key in m && val in m[key] ==> key in m' && val in m'[key]
+    //   //  k is added to the tuples of xe
+    //   ensures forall e:: e in xe ==> e in m' && k in m'[e]
+    //   //  A key in m' is either in m or in xe
+    //   ensures forall key:: key in m' <==> key in m || key in xe
+    //   ensures forall key:: key in m' <==> 0 <= key < b
+    //   ensures forall key, i:: key in m' && 0 <= i < |m'[key]| ==> 0 <= m'[key][i] < b
+
+    //    //  A value in m' is either in m[key] or k
+    //   ensures forall key, val:: key in m' && val in m'[key] <==> ((key in m && val in m[key]) || (val == k && key in xe))
+    // {
+    //   if |xe| == 0 then m
+    //   else
+    //     var m1 := m[xe[0] := m[xe[0]] + [k]];
+    //     // assert forall key, val:: key in m && val in m[key] ==> key in m1 && val in m1[key];
+    //     // assert forall key, i:: key in m1 && 0 <= i < |m1[key]| ==> 0 <= m1[key][i] < b;
+    //     AddReverseEntries(m[xe[0] := m[xe[0]] + [k]], k, xe[1..], b)
+    // }
+
+
 
     /**
       * Returns the number of states of the automaton.
@@ -170,7 +388,7 @@ module Automata {
     /**
       *  The number of transitions.
       */
-    function {:opaque} TSize(index: nat := 0): nat
+    function {:opaque} TSize(index: nat := 0): nat 
       requires this.IsValid()
       requires index <= |states|
       decreases |states| - index
@@ -230,25 +448,121 @@ module Automata {
       print "}\n";
     }
 
+    // function {:timeLimitMultiplier 2} ReverseAuto(index: nat := 0, a: ValidAuto<T>): (a': ValidAuto<T>)
+    //   requires this.IsValid()
+    //   requires index <= |states|
+    //   requires a.states == states
+    //   requires forall j, tgt:: 0 <= j < index && tgt in transitions[states[j]] ==> (states[j] in a.transitions[tgt])
+    //   ensures a'.states == states
+    //   //   ensures forall j, tgt:: j in  states && tgt in transitions[j] ==> (j in a'.transitions[tgt])
+    //   ensures forall j, tgt:: 0 <= j < |states| && tgt in transitions[states[j]] ==> (states[j] in a'.transitions[tgt])
+
+    //   decreases |states| - index
+    // {
+    //   //   reveal_AddReverseEdges();
+    //   //   reveal_AddStates();
+    //   if |states| == index then a
+    //   else
+    //     var aut2 := a.AddReverseEdges(
+    //                   states[index],
+    //                   MapP(transitionsNat[index], i requires i in transitionsNat[index] => states[i]));
+    //     // assert forall j:: 0 <= j < |js| ==> i in a.transitions[js[j]];
+    //     assume  forall j, tgt:: 0 <= j < index + 1 && tgt in transitions[states[j]] ==> (states[j] in aut2.transitions[tgt]);
+    //     ReverseAuto(index + 1, aut2)
+    // }
+
     /**
       * Check if the automaton is valid.
       */
     ghost predicate IsValid() {
+      //   && (forall i : T :: i in states <==> i in transitions)
+      //   && (forall k, k':: 0 <= k < k' < |states| ==> states[k] != states[k'])
+      //   && (forall i, j :: i in states && 0 <= j < |transitions[i]| ==> transitions[i][j] in states)
+      && StatesTransValid()
+
+      //   && (forall s:: s in states <==> s in indexOf)
+      //   && (forall i:: i in indexOf ==> indexOf[i] < |states| && states[indexOf[i]] == i)
+      //   && (forall i:: 0 <= i < |states| ==> states[i] in indexOf && indexOf[states[i]] == i)
+      //   && (indexOf.Values == set z {:nowarn} | 0 <= z < |states|)
+      //   && (indexOf.Values == transitionsNat.Keys)
+      && IndexOfValid()
+
+      //   && (forall k:: k in transitionsNat ==> |transitionsNat[k]| == |transitions[states[k]]|)
+      //   && (forall k:: k in transitions ==> |transitions[k]| == |transitionsNat[indexOf[k]]|)
+      //   && (forall i, j :: 0 <= i < |states| && 0 <= j < |transitionsNat[i]| ==> 0 <= transitionsNat[i][j] < |states|)
+      //   && ((forall i, j :: 0 <= i < |states| && 0 <= j < |transitionsNat[i]| ==> states[transitionsNat[i][j]] == transitions[states[i]][j]))
+      //   && ((forall i:T , j :: i in states && 0 <= j < |transitions[i]| ==> indexOf[transitions[i][j]] == indexOf[transitions[i][j]]))
+      && TransNatTransIsValid()
+
+      //   && transitionsNat.Keys == revTransitionsNat.Keys
+      //        && (forall src, tgt:: src in transitionsNat && tgt in transitionsNat[src]
+      //                              ==> tgt in revTransitionsNat && src in revTransitionsNat[tgt])
+      //   && (forall src, tgt:: src in revTransitionsNat && tgt in revTransitionsNat[src]
+      //                         ==> tgt in transitionsNat && src in transitionsNat[tgt])
+      //   && IsReversemap(transitionsNat, revTransitionsNat)
+    }
+
+    ghost predicate StatesTransValid() {
       && (forall i : T :: i in states <==> i in transitions)
       && (forall k, k':: 0 <= k < k' < |states| ==> states[k] != states[k'])
       && (forall i, j :: i in states && 0 <= j < |transitions[i]| ==> transitions[i][j] in states)
+    }
+
+    ghost predicate IndexOfValid()
+    {
       && (forall s:: s in states <==> s in indexOf)
       && (forall i:: i in indexOf ==> indexOf[i] < |states| && states[indexOf[i]] == i)
       && (forall i:: 0 <= i < |states| ==> states[i] in indexOf && indexOf[states[i]] == i)
       && (indexOf.Values == set z {:nowarn} | 0 <= z < |states|)
       && (indexOf.Values == transitionsNat.Keys)
-         //   && (transitionsNat.Keys == set z {:nowarn} | 0 <= z < |states|)
+      && (indexOf.Values == revTransitionsNat.Keys)
+    }
 
+    ghost predicate TransNatTransIsValid()
+      requires StatesTransValid()
+      requires IndexOfValid()
+    {
       && (forall k:: k in transitionsNat ==> |transitionsNat[k]| == |transitions[states[k]]|)
       && (forall k:: k in transitions ==> |transitions[k]| == |transitionsNat[indexOf[k]]|)
       && (forall i, j :: 0 <= i < |states| && 0 <= j < |transitionsNat[i]| ==> 0 <= transitionsNat[i][j] < |states|)
       && ((forall i, j :: 0 <= i < |states| && 0 <= j < |transitionsNat[i]| ==> states[transitionsNat[i][j]] == transitions[states[i]][j]))
       && ((forall i:T , j :: i in states && 0 <= j < |transitions[i]| ==> indexOf[transitions[i][j]] == indexOf[transitions[i][j]]))
     }
+
+    ghost predicate IsReversemapValid()
+    {
+      //   && transitionsNat.Keys == revTransitionsNat.Keys
+      && (forall src, tgt:: src in transitionsNat && tgt in transitionsNat[src]
+                            <==> tgt in revTransitionsNat && src in revTransitionsNat[tgt])
+    }
+
+    ghost predicate IsReversemapValid2()
+    {
+      IsReversemap(transitionsNat, revTransitionsNat)
+      //   && m.Keys == m'.Keys
+      //   && (forall src, tgt:: src in m && tgt in m[src]
+      //                         ==> tgt in m' && src in m'[tgt])
+      //   && (forall src, tgt:: src in m' && tgt in m'[src]
+      //                         ==> tgt in m && src in m[tgt])
+    }
+
+    static ghost predicate IsReversemap(m: map<nat, seq<nat>>, m': map<nat, seq<nat>>)
+    {
+      && m.Keys == m'.Keys
+      && (forall src, tgt:: src in m && tgt in m[src]
+                            <==> tgt in m' && src in m'[tgt])
+         //   && (forall src, tgt:: src in m' && tgt in m'[src]
+         //                         ==> tgt in m && src in m[tgt])
+    }
+
+    static ghost predicate IsReversemap2<T>(m: map<T, seq<T>>, m': map<T, seq<T>>)
+    {
+      && m.Keys == m'.Keys
+      && (forall src, tgt:: src in m && tgt in m[src]
+                            ==> tgt in m' && src in m'[tgt])
+         //   && (forall src, tgt:: src in m' && tgt in m'[src]
+         //                         ==> tgt in m && src in m[tgt])
+    }
+
   }
 }
